Replaced all occurences of SIMP with pure

coq-osiris/theories/proofmode/capital_SIMP.v
@@ -15,25 +15,22 @@ From osiris.proofmode Require Import notations.
 
 (* -------------------------------------------------------------------------- *)
 
-(* The judgement [SIMP m φ] asserts that the computation [m] can be simplified
+(* The judgement [pure m φ] asserts that the computation [m] can be simplified
    to [ret #x], where [x] is a (logical) value so that [φ x] holds. *)
 
 (* Because the relation [simp] is inductively defined, this judgement implies
    that [m] terminates. This is a Hoare logic of total correctness. *)
 
-Definition SIMP `{Encode X} (m : micro val) (φ : X → Prop) :=
-  ∃ x, simp m (ret #x) ∧ φ x.
-
 (* -------------------------------------------------------------------------- *)
 
 (* Basic reasoning rules for [ret], [bind], [try]. *)
 
-Lemma SIMP_ret `{Encode X} (φ : X → Prop) v x :
+Lemma pure_ret `{Encode X} (φ : X → Prop) v x :
   v = #x →
   φ x →
-  SIMP (ret v) φ.
+  pure (ret v) φ.
 Proof.
-  unfold SIMP. intros. subst. eauto with simp.
+  unfold pure. intros. subst. eauto with simp.
 Qed.
 
 (* A reasoning rule for [try]. *)
@@ -41,11 +38,11 @@ Qed.
 (* The rule is degenerate; [m] is not allowed to reduce to [Next],
    so the handler [g] is dead and no proof obligation bears on it. *)
 
-Lemma SIMP_try X (_ : Encode X) Y (_ : Encode Y)
+Lemma pure_try X (_ : Encode X) Y (_ : Encode Y)
   m f g (φ : X → Prop) (ψ : Y → Prop) :
-  SIMP m φ →
-  (∀ x, φ x → SIMP (f #x) ψ) →
-  SIMP (try m f g) ψ.
+  pure m φ →
+  (∀ x, φ x → pure (f #x) ψ) →
+  pure (try m f g) ψ.
 Proof.
   intros (x & ? & Hx) Hf.
   specialize (Hf x Hx).
@@ -57,13 +54,13 @@ Qed.
 
 (* This is [@bind val val]. *)
 
-Lemma SIMP_bind X (_ : Encode X) Y (_ : Encode Y)
+Lemma pure_bind X (_ : Encode X) Y (_ : Encode Y)
   m f (φ : X → Prop) (ψ : Y → Prop) :
-  SIMP m φ →
-  (∀ x, φ x → SIMP (f #x) ψ) →
-  SIMP (bind m f) ψ.
+  pure m φ →
+  (∀ x, φ x → pure (f #x) ψ) →
+  pure (bind m f) ψ.
 Proof.
-  rewrite bind_as_try. eauto using SIMP_try.
+  rewrite bind_as_try. eauto using pure_try.
 Qed.
 
 (* This Iris-style variant of the Bind rule has just one premise. It is
@@ -71,20 +68,20 @@ Qed.
 
 (* This is [@bind val val]. *)
 
-Lemma SIMP_bind_unary X (_ : Encode X) Y (_ : Encode Y)
+Lemma pure_bind_unary X (_ : Encode X) Y (_ : Encode Y)
   m f (ψ : Y → Prop) :
-  SIMP m (λ (x : X), SIMP (f #x) ψ) ->
-  SIMP (bind m f) ψ.
+  pure m (λ (x : X), pure (f #x) ψ) ->
+  pure (bind m f) ψ.
 Proof.
-  eauto using SIMP_bind.
+  eauto using pure_bind.
 Qed.
 
-Lemma SIMP_prove_bind_bind `{Encode A} `{Encode X} m (a : A)
+Lemma pure_prove_bind_bind `{Encode A} `{Encode X} m (a : A)
   (f : A -> micro val) (g : val -> micro val) (φ : X -> Prop) :
   simp ('c ← m;
         f c) (ret #a) ->
-  SIMP (g #a) φ ->
-  SIMP ('v1 ← m;
+  pure (g #a) φ ->
+  pure ('v1 ← m;
         'v2 ← f v1;
         g v2) φ.
 Proof.
@@ -96,55 +93,55 @@ Proof.
   done.
 Qed.
   
-Lemma SIMP_bind_bind `{Encode X} `{Encode Y} (m : micro val) f g
+Lemma pure_bind_bind `{Encode X} `{Encode Y} (m : micro val) f g
   (φ : X -> Prop) (ψ : Y -> Prop) :
-  SIMP ('x ← m;
+  pure ('x ← m;
         f x) ψ ->
-  (forall y, ψ y -> SIMP (g #y) φ) ->
-  SIMP ('x ← m;
+  (forall y, ψ y -> pure (g #y) φ) ->
+  pure ('x ← m;
         y ← f x;
         g y) φ.
 Proof.
   intros (x & Hsimp & ?) ?.
-  eapply SIMP_prove_bind_bind; first apply Hsimp.
+  eapply pure_prove_bind_bind; first apply Hsimp.
   rewrite <- solve_encode_val.
   auto.
 Qed.
 
-Lemma SIMP_bind_binary `{Encode X} `{Encode Y} (m : micro val) f g
+Lemma pure_bind_binary `{Encode X} `{Encode Y} (m : micro val) f g
   (φ : X -> Prop) (ψ : Y -> Prop) :
-  SIMP m (fun x => SIMP (f x) ψ) ->
-  (forall y, ψ y -> SIMP (g #y) φ) ->
-  SIMP ('x ← m;
+  pure m (fun x => pure (f x) ψ) ->
+  (forall y, ψ y -> pure (g #y) φ) ->
+  pure ('x ← m;
         y ← f x;
         g y) φ.
 Proof.
   intros.
-  eapply SIMP_bind_bind; first eapply SIMP_bind; eauto.
+  eapply pure_bind_bind; first eapply pure_bind; eauto.
   intros; auto.
 Qed.
 
 (* -------------------------------------------------------------------------- *)
 
-(* This lemma allows simplifying a goal of the form [SIMP m φ] by first
+(* This lemma allows simplifying a goal of the form [pure m φ] by first
    simplifying [m] into [m'], then reasoning about [m']. *)
 
-Lemma SIMP_simp `{Encode X} m m' (φ : X → Prop) :
+Lemma pure_simp `{Encode X} m m' (φ : X → Prop) :
   simp m m' →
-  SIMP m' φ →
-  SIMP m φ.
+  pure m' φ →
+  pure m φ.
 Proof.
-  unfold SIMP.
+  unfold pure.
   intros ? (x & ? & ?).
   eauto with simp.
 Qed.
 
 (* The Consequence rule. *)
 
-Lemma SIMP_covariant `{Encode X} m (φ ψ : X → Prop) :
-  SIMP m φ →
+Lemma pure_covariant `{Encode X} m (φ ψ : X → Prop) :
+  pure m φ →
   (∀ x, φ x → ψ x) →
-  SIMP m ψ.
+  pure m ψ.
 Proof.
   intros (x & Hm & Hx) ?. exists x. eauto.
 Qed.
@@ -162,11 +159,11 @@ Proof.
   destruct x; eauto using prove_simp_bind with simp.
 Qed.
 
-Lemma SIMP_bind_as_bool Y (_ : Encode Y)
+Lemma pure_bind_as_bool Y (_ : Encode Y)
   m (f : bool → micro val) (φ : bool → Prop) (ψ : Y → Prop) :
-  SIMP m φ →
-  (∀ (x : bool), φ x → SIMP (f x) ψ) →
-  SIMP (bind (as_bool m) f) ψ.
+  pure m φ →
+  (∀ (x : bool), φ x → pure (f x) ψ) →
+  pure (bind (as_bool m) f) ψ.
   (* This is [@bind bool val]. *)
 Proof.
   intros (x & ? & Hx) Hf.
@@ -184,11 +181,11 @@ Proof.
   eauto using prove_simp_bind with simp.
 Qed.
 
-Lemma SIMP_bind_as_int Y (_ : Encode Y)
+Lemma pure_bind_as_int Y (_ : Encode Y)
   m (f : int → micro val) (φ : Z → Prop) (ψ : Y → Prop) :
-  SIMP m φ →
-  (∀ (x : Z), φ x → SIMP (f (repr x)) ψ) →
-  SIMP (bind (as_int m) f) ψ.
+  pure m φ →
+  (∀ (x : Z), φ x → pure (f (repr x)) ψ) →
+  pure (bind (as_int m) f) ψ.
   (* This is [@bind int val]. *)
 Proof.
   intros (x & ? & Hx) Hf.
@@ -207,25 +204,25 @@ Qed.
    subgoal instantiates both the metavariable [x] and the metavariable [X],
    which is the type of [x]. *)
 
-Lemma SIMP_call `{Encode X} `{Encode Y}
+Lemma pure_call `{Encode X} `{Encode Y}
   (φ : Y → Prop) v1 v'2 (x : X) :
   v'2 = #x →
-  SIMP (call v1 #x) φ →
-  SIMP (call v1 v'2) φ.
+  pure (call v1 #x) φ →
+  pure (call v1 v'2) φ.
 Proof.
   intros. subst. eauto.
 Qed.
 
-(* This lemma combines [SIMP_covariant] and [SIMP_call]. *)
+(* This lemma combines [pure_covariant] and [pure_call]. *)
 
-Lemma SIMP_call_covariant `{Encode X} `{Encode Y}
+Lemma pure_call_covariant `{Encode X} `{Encode Y}
   (φ ψ : Y → Prop) v1 v'2 (x : X) :
   v'2 = #x →
-  SIMP (call v1 #x) φ →
+  pure (call v1 #x) φ →
   (∀ y, φ y → ψ y) →
-  SIMP (call v1 v'2) ψ.
+  pure (call v1 v'2) ψ.
 Proof.
-  eauto using SIMP_covariant, SIMP_call.
+  eauto using pure_covariant, pure_call.
 Qed.
 
 (* The following two lemmas paraphrase the definition of [call] in eval.v.
@@ -233,52 +230,52 @@ Qed.
    a concrete closure (as opposed to a rigid metavariable), they step into
    the call. *)
 
-Lemma SIMP_enter_call_VClo `{Encode Y} η a v2 (φ : Y → Prop) :
-  SIMP (acall η a v2) φ ->
-  SIMP (call (VClo η a) v2) φ.
+Lemma pure_enter_call_VClo `{Encode Y} η a v2 (φ : Y → Prop) :
+  pure (acall η a v2) φ ->
+  pure (call (VClo η a) v2) φ.
 Proof.
   tauto.
 Qed.
 
-Lemma SIMP_enter_call_VCloRec `{Encode Y} η rbs g v2 (φ : Y → Prop) :
-  SIMP (
+Lemma pure_enter_call_VCloRec `{Encode Y} η rbs g v2 (φ : Y → Prop) :
+  pure (
     let δ := eval_rec_bindings η rbs in
     let η := concat δ η in
     a ← lookup_rec_bindings rbs g ;
     acall η a v2
   ) φ ->
-  SIMP (call (VCloRec η rbs g) v2) φ.
+  pure (call (VCloRec η rbs g) v2) φ.
 Proof.
   tauto.
 Qed.
 
-Lemma SIMP_call_VCloRec `{Encode Y} η rbs g v2 (φ : Y → Prop) :
-  SIMP (
+Lemma pure_call_VCloRec `{Encode Y} η rbs g v2 (φ : Y → Prop) :
+  pure (
     let δ := eval_rec_bindings η rbs in
     let η := concat δ η in
     a ← lookup_rec_bindings rbs g ;
     acall η a v2
   ) φ =
-  SIMP (call (VCloRec η rbs g) v2) φ.
+  pure (call (VCloRec η rbs g) v2) φ.
 Proof.
   tauto.
 Qed.
 
-Lemma invert_SIMP_crash `{Encode Y} (φ : Y -> Prop) :
-  SIMP Crash φ -> False.
+Lemma invert_pure_crash `{Encode Y} (φ : Y -> Prop) :
+  pure Crash φ -> False.
 Proof.
   intros (? & Hsimp & _).
   by apply simp_crash_ret in Hsimp.
 Qed.
 
-Lemma invert_SIMP_call `{Encode Y} f v (φ : Y -> Prop) : 
-  SIMP (call f v) φ ->
+Lemma invert_pure_call `{Encode Y} f v (φ : Y -> Prop) : 
+  pure (call f v) φ ->
   (exists η a, f = VClo η a) \/ exists η rbs g, f = VCloRec η rbs g. 
 Proof.
   intros Hcall.
   unfold call in Hcall.
   destruct f; simpl in Hcall;
-    ((exfalso; by eapply invert_SIMP_crash) || eauto).
+    ((exfalso; by eapply invert_pure_crash) || eauto).
 Qed.
 
 (* Replace the first occurence of a var in an environment *)
@@ -381,25 +378,25 @@ Proof.
   rewrite replace_env_idempotent; auto.
 Qed.
 
-Lemma SIMP_Eval `{Encode X} η e k ko (φ : X -> Prop) :
-  SIMP (try (eval η e) k ko) φ ->
-  SIMP (Stop CEval (η, e) k ko) φ.
+Lemma pure_Eval `{Encode X} η e k ko (φ : X -> Prop) :
+  pure (try (eval η e) k ko) φ ->
+  pure (Stop CEval (η, e) k ko) φ.
 Proof.
   intros.
-  by eapply SIMP_simp; first apply SimpEval.
+  by eapply pure_simp; first apply SimpEval.
 Qed.
 
-Lemma SIMP_EvalRetNext `{Encode X} η e (φ : X -> Prop) :
-  SIMP (eval η e) φ ->
-  SIMP (Stop CEval (η, e) ret (fun _ => Next)) φ.
+Lemma pure_EvalRetNext `{Encode X} η e (φ : X -> Prop) :
+  pure (eval η e) φ ->
+  pure (Stop CEval (η, e) ret (fun _ => Next)) φ.
 Proof.
   intros.
-  by eapply SIMP_simp; [apply advance_SimpEvalRetNext; apply SimpReflexive|].
+  by eapply pure_simp; [apply advance_SimpEvalRetNext; apply SimpReflexive|].
 Qed.
 
 (* (* Todo: write comment *) *)
 
-Lemma SIMP_rec_call `{Encode X} `{Encode Y}
+Lemma pure_rec_call `{Encode X} `{Encode Y}
   (η : env) (rbs : rec_bindings) (fname : var) (v : X)
   (P : X -> Prop) (φ : X -> Y -> Prop) (R : X -> X -> Prop) :
   well_founded R ->
@@ -409,24 +406,24 @@ Lemma SIMP_rec_call `{Encode X} `{Encode Y}
       (forall v'',
           P v'' ->
           R v'' v' ->
-          SIMP (call vf #v'') (φ v'')) ->
-      SIMP ('afun ← lookup_rec_bindings rbs fname ;
+          pure (call vf #v'') (φ v'')) ->
+      pure ('afun ← lookup_rec_bindings rbs fname ;
             let δ := replace_env_binding (eval_rec_bindings η rbs) fname vf in
             let 'AnonFun x e := afun in
             eval (EnvCons x #v' (concat δ η)) e
         ) (φ v')) ->
-  SIMP (call (VCloRec η rbs fname) #v) (φ v).
+  pure (call (VCloRec η rbs fname) #v) (φ v).
 Proof.
   intros Hwf HP Hrec.
   induction v as [v IH] using (well_founded_induction Hwf); intros.
-  apply SIMP_enter_call_VCloRec; simpl in *.
+  apply pure_enter_call_VCloRec; simpl in *.
   destruct (lookup_rec_bindings_cases rbs fname) as [Hlkp|[afun Hlkp]].
   { rewrite Hlkp in *; simpl in *.
     eapply Hrec with (vf:=VInt int.zero); eauto. }
   { specialize (Hrec (VCloRec η rbs fname) v HP).
     erewrite replace_binding in Hrec by eauto.
     simpl in *; rewrite !Hlkp in *; simpl in *.
-    unfold acall; destruct afun; apply SIMP_EvalRetNext.
+    unfold acall; destruct afun; apply pure_EvalRetNext.
     eapply Hrec; auto. }
 Qed.
 
@@ -440,7 +437,7 @@ Notation "'RecBinds' x ; y ; .. ; z" :=
     (at level 60,
       format "'RecBinds'  x ;  '/' y ; '/' .. ; '/' z").
 
-Lemma SIMP_rec_call_unary `{Encode X} `{Encode Y}
+Lemma pure_rec_call_unary `{Encode X} `{Encode Y}
   (η : env) afun (fname : var) (v : X)
   (P : X -> Prop) (φ : X -> Y -> Prop) (R : X -> X -> Prop) :
   well_founded R ->
@@ -450,25 +447,25 @@ Lemma SIMP_rec_call_unary `{Encode X} `{Encode Y}
       (forall v'',
           P v'' ->
           R v'' v' ->
-          SIMP (call vf #v'') (φ v'')) -> 
-      SIMP (let 'AnonFun x e := afun in
+          pure (call vf #v'') (φ v'')) -> 
+      pure (let 'AnonFun x e := afun in
             eval (EnvCons x #v' (EnvCons fname vf η)) e) (φ v')) ->
-  SIMP (call (VCloRec η (RecBind fname to afun) fname) #v) (φ v).
+  pure (call (VCloRec η (RecBind fname to afun) fname) #v) (φ v).
 Proof.
 (*   intros Hwf HP Hrec. *)
-(*   eapply SIMP_rec_call. *)
+(*   eapply pure_rec_call. *)
 (*   { apply Hwf. } *)
 (*   { apply HP. } *)
 (*   simpl; rewrite String.eqb_refl. apply Hrec. *)
 (* Qed. *)
   intros Hwf HP Hrec.
   induction v as [v IH] using (well_founded_induction Hwf); intros.
-  apply SIMP_enter_call_VCloRec; simpl; rewrite String.eqb_refl.
-  unfold acall; destruct afun; apply SIMP_EvalRetNext.
+  apply pure_enter_call_VCloRec; simpl; rewrite String.eqb_refl.
+  unfold acall; destruct afun; apply pure_EvalRetNext.
   eapply Hrec; auto.
 Qed.
 
-Lemma SIMP_rec_call_binary_mutual `{Encode X} `{Encode Y}
+Lemma pure_rec_call_binary_mutual `{Encode X} `{Encode Y}
   (η : env) (afun agun : anonfun) (gname fname : var) (v : X)
   (P : X -> Prop) (φ : X -> Y -> Prop) (R : X -> X -> Prop) :
   well_founded R ->
@@ -478,28 +475,28 @@ Lemma SIMP_rec_call_binary_mutual `{Encode X} `{Encode Y}
       (forall v'',
           P v'' ->
           R v'' v' ->
-          SIMP (call vf #v'') (φ v'')) -> 
-      SIMP (let 'AnonFun x e := afun in
+          pure (call vf #v'') (φ v'')) -> 
+      pure (let 'AnonFun x e := afun in
             eval (x ~> #v';
                   fname ~> vf;
                   gname ~> (VCloRec η (RecBinds fname to afun; gname to agun) gname);
                   η) e) (φ v')) ->
-  SIMP (call (VCloRec η (RecBinds fname to afun; gname to agun) fname) #v) (φ v).
+  pure (call (VCloRec η (RecBinds fname to afun; gname to agun) fname) #v) (φ v).
 Proof.
 (*   intros Hwf HP Hrec. *)
-(*   eapply SIMP_rec_call. *)
+(*   eapply pure_rec_call. *)
 (*   { apply Hwf. } *)
 (*   { apply HP. } *)
 (*   simpl; rewrite String.eqb_refl. apply Hrec. *)
 (* Qed. *)
   intros Hwf HP Hrec.
   induction v as [v IH] using (well_founded_induction Hwf); intros.
-  apply SIMP_enter_call_VCloRec; simpl; rewrite String.eqb_refl.
-  unfold acall; destruct afun; apply SIMP_EvalRetNext.
+  apply pure_enter_call_VCloRec; simpl; rewrite String.eqb_refl.
+  unfold acall; destruct afun; apply pure_EvalRetNext.
   eapply Hrec; auto.
 Qed.
 
-Lemma SIMP_rec_call_binary_mutual_aliasing `{Encode X} `{Encode Y}
+Lemma pure_rec_call_binary_mutual_aliasing `{Encode X} `{Encode Y}
   (η : env) ef eg farg garg (gname fname : var) (v : X)
   (P : X -> Prop) (φ : X -> Y -> Prop) (R : X -> X -> Prop) :
   well_founded R ->
@@ -509,8 +506,8 @@ Lemma SIMP_rec_call_binary_mutual_aliasing `{Encode X} `{Encode Y}
       (forall v'',
           P v'' ->
           R v'' v' ->
-          SIMP (call vf #v'') (φ v'')) -> 
-      SIMP (eval ((if (fname =? gname)%string then garg else farg) ~> #v';
+          pure (call vf #v'') (φ v'')) -> 
+      pure (eval ((if (fname =? gname)%string then garg else farg) ~> #v';
                   gname ~>
                     if (fname =? gname)%string
                     then vf
@@ -528,10 +525,10 @@ Lemma SIMP_rec_call_binary_mutual_aliasing `{Encode X} `{Encode Y}
                             fname)
                     else vf;
                   η) (if (fname =? gname)%string then eg else ef)) (φ v')) ->
-  SIMP (call (VCloRec η (RecBinds gname to (AnonFun garg eg); fname to (AnonFun farg ef)) fname) #v) (φ v).
+  pure (call (VCloRec η (RecBinds gname to (AnonFun garg eg); fname to (AnonFun farg ef)) fname) #v) (φ v).
 Proof.
 (*   intros Hwf HP Hrec. *)
-(*   eapply SIMP_rec_call. *)
+(*   eapply pure_rec_call. *)
 (*   { apply Hwf. } *)
 (*   { apply HP. } *)
 (*   simpl; destruct (fname =? gname)%string eqn:name_eq; simpl. *)
@@ -540,13 +537,13 @@ Proof.
 (* Qed. *)
   intros Hwf HP Hrec.
   induction v as [v IH] using (well_founded_induction Hwf); intros.
-  apply SIMP_enter_call_VCloRec; simpl; rewrite String.eqb_refl.
-  unfold acall; destruct (fname =? gname)%string eqn:name_eq; apply SIMP_EvalRetNext.
+  apply pure_enter_call_VCloRec; simpl; rewrite String.eqb_refl.
+  unfold acall; destruct (fname =? gname)%string eqn:name_eq; apply pure_EvalRetNext.
   { apply String.eqb_eq in name_eq as ->. eapply Hrec; eauto. }
   eapply Hrec; eauto.
 Qed.
 
-Lemma SIMP_rec_call_binary_mutual2 `{Encode X} `{Encode Y}
+Lemma pure_rec_call_binary_mutual2 `{Encode X} `{Encode Y}
   (η : env) ef farg agun (gname fname : var) (v : X)
   (P : X -> Prop) (φ : X -> Y -> Prop) (R : X -> X -> Prop) :
   well_founded R ->
@@ -557,16 +554,16 @@ Lemma SIMP_rec_call_binary_mutual2 `{Encode X} `{Encode Y}
       (forall v'',
           P v'' ->
           R v'' v' ->
-          SIMP (call vf #v'') (φ v'')) -> 
-      SIMP (eval (farg ~> #v';
+          pure (call vf #v'') (φ v'')) -> 
+      pure (eval (farg ~> #v';
                   gname ~>
                     (VCloRec η (RecBinds gname to agun; fname to (AnonFun farg ef)) gname);
                   fname ~> vf;
                   η) ef) (φ v')) ->
-  SIMP (call (VCloRec η (RecBinds gname to agun; fname to (AnonFun farg ef)) fname) #v) (φ v).
+  pure (call (VCloRec η (RecBinds gname to agun; fname to (AnonFun farg ef)) fname) #v) (φ v).
 Proof.
 (*   intros Hwf HP Hname Hrec. *)
-(*   eapply SIMP_rec_call. *)
+(*   eapply pure_rec_call. *)
 (*   { apply Hwf. } *)
 (*   { apply HP. } *)
 (*   simpl. rewrite Hname. rewrite String.eqb_refl. simpl. *)
@@ -574,16 +571,16 @@ Proof.
   (* Qed. *)
   intros Hwf HP Hname Hrec.
   induction v as [v IH] using (well_founded_induction Hwf); intros.
-  apply SIMP_enter_call_VCloRec; simpl; rewrite String.eqb_refl.
-  unfold acall; rewrite Hname; apply SIMP_EvalRetNext.
+  apply pure_enter_call_VCloRec; simpl; rewrite String.eqb_refl.
+  unfold acall; rewrite Hname; apply pure_EvalRetNext.
   eapply Hrec; eauto.
 Qed.
 
-Definition nested_SIMP `{Encode X} vf arg1 arg2 (φ : X -> Prop) :=
-  SIMP (call vf arg1) (fun c =>
-                         SIMP (call c arg2) φ).
+Definition nested_pure `{Encode X} vf arg1 arg2 (φ : X -> Prop) :=
+  pure (call vf arg1) (fun c =>
+                         pure (call c arg2) φ).
 
-Lemma SIMP_nested_rec_call `{Encode A} `{Encode B} `{Encode C}
+Lemma pure_nested_rec_call `{Encode A} `{Encode B} `{Encode C}
   (η : env) farg farg2 ef ef2 (fname : var) (v1 : A) (v2 : B)
   (P : A -> B -> Prop) (φ : A -> B -> C -> Prop) (R : (A * B) -> (A * B) -> Prop) :
   let vclo := (VCloRec η (RecBind fname to (AnonFun farg ef)) fname) in
@@ -598,10 +595,10 @@ Lemma SIMP_nested_rec_call `{Encode A} `{Encode B} `{Encode C}
           eval η1' ef = ret (VClo η1' (AnonFun farg2 ef2)) ->
           P v1'' v2'' ->
           R (v1'', v2'') (v1', v2') ->
-          nested_SIMP vf #v1'' #v2'' (φ v1'' v2'')) ->
+          nested_pure vf #v1'' #v2'' (φ v1'' v2'')) ->
       let δ := (farg2 ~> #v2'; farg ~> #v1'; fname ~> vf; η) in
-      SIMP (eval δ ef2) (φ v1' v2')) ->
-  nested_SIMP vclo #v1 #v2 (φ v1 v2).
+      pure (eval δ ef2) (φ v1' v2')) ->
+  nested_pure vclo #v1 #v2 (φ v1 v2).
 Proof.
   cbn zeta.
   intros Hwf HP Heval Hrec.
@@ -611,16 +608,16 @@ Proof.
   clear v1 v2 Hpeq.
   induction p as [p IH] using (well_founded_induction Hwf); intros.
   destruct p as [v1 v2]; simpl in *.
-  apply SIMP_enter_call_VCloRec; simpl; rewrite String.eqb_refl; simpl.
+  apply pure_enter_call_VCloRec; simpl; rewrite String.eqb_refl; simpl.
   
-  unfold acall; apply SIMP_EvalRetNext.
-  rewrite Heval. eapply SIMP_ret; first solve [encode].
-  apply SIMP_enter_call_VClo; simpl; apply SIMP_EvalRetNext.
+  unfold acall; apply pure_EvalRetNext.
+  rewrite Heval. eapply pure_ret; first solve [encode].
+  apply pure_enter_call_VClo; simpl; apply pure_EvalRetNext.
   eapply Hrec; auto; intros.
   apply (IH (v1'', v2'')); auto.
 Qed.
 
-Lemma SIMP_nested_call `{Encode A} `{Encode B} `{Encode C}
+Lemma pure_nested_call `{Encode A} `{Encode B} `{Encode C}
   (η : env) rbs (fname : var) (v1 : A) (v2 : B) x y e1 e2
   (P : A -> B -> Prop) (φ : A -> B -> C -> Prop) (R : (A * B) -> (A * B) -> Prop) :
   let δ := eval_rec_bindings η rbs in
@@ -636,10 +633,10 @@ Lemma SIMP_nested_call `{Encode A} `{Encode B} `{Encode C}
            eval η0 e1 = ret (VClo η0 (AnonFun y e2))) ->
           P v1'' v2'' ->
           R (v1'', v2'') (v1', v2') ->
-          nested_SIMP vf #v1'' #v2'' (φ v1'' v2'')) ->
+          nested_pure vf #v1'' #v2'' (φ v1'' v2'')) ->
       let δ := replace_env_binding δ fname vf in
-      SIMP (eval (y ~> #v2'; x ~> #v1'; concat δ η) e2) (φ v1' v2')) ->
-  nested_SIMP (VCloRec η rbs fname) #v1 #v2 (φ v1 v2).
+      pure (eval (y ~> #v2'; x ~> #v1'; concat δ η) e2) (φ v1' v2')) ->
+  nested_pure (VCloRec η rbs fname) #v1 #v2 (φ v1 v2).
 Proof.
   cbn zeta.
   intros Hlkp Heval Hwf HP Hrec.
@@ -649,10 +646,10 @@ Proof.
   clear v1 v2 Hpeq.
   induction p as [p IH] using (well_founded_induction Hwf); intros.
   destruct p as [v1 v2]; simpl in *.
-  apply SIMP_enter_call_VCloRec; rewrite Hlkp; simpl.
-  apply SIMP_EvalRetNext. rewrite Heval.
-  eapply SIMP_ret; first solve [encode].
-  apply SIMP_enter_call_VClo; apply SIMP_EvalRetNext.
+  apply pure_enter_call_VCloRec; rewrite Hlkp; simpl.
+  apply pure_EvalRetNext. rewrite Heval.
+  eapply pure_ret; first solve [encode].
+  apply pure_enter_call_VClo; apply pure_EvalRetNext.
   rewrite <- (replace_binding _ _ _ _ Hlkp). 
   eapply Hrec; auto; intros.
   apply (IH (v1'', v2'')); auto.
